proof lhole

src/syncablep.lean
@@ -8,13 +8,13 @@ variables {n : ℕ} {σ : Type} {ι : Type} {τ : ι → Type} [decidable_eq ι]
 
 /-- syncable with the exception that no thread is allowed to store 
 or load in stores and loads respectively. Adding to stores or load makes this property stricter -/
-def syncable' (stores : set ι) (loads : set ι) (s : state n σ τ) (m : memory τ) : Prop :=
+def syncable' (shole : set ι) (lhole : set ι) (s : state n σ τ) (m : memory τ) : Prop :=
 (∀i:ι,
     (∀ tid, i ∉ (s.threads.nth tid).stores ∧ m i = (s.threads.nth tid).global i) ∨
     (∃ tid, i ∈ (s.threads.nth tid).stores ∧ m i = (s.threads.nth tid).global i ∧
         (∀ tid', tid ≠ tid' → i ∉ (s.threads.nth tid').accesses))) ∧
-(∀ i tid, i ∈ stores → i ∉ (s.threads.nth tid).stores) ∧
-(∀ i tid, i ∈ loads → i ∉ (s.threads.nth tid).loads)
+(∀ i tid, (i ∈ shole → i ∉ (s.threads.nth tid).stores) ∧
+        (i ∈ lhole → i ∉ (s.threads.nth tid).loads))
 
 example (s : state n σ τ) (m : memory τ) : syncable' ∅ ∅ s m ↔ state.syncable s m := begin
     unfold syncable',
